Weakest pre-condition

Hoare2.v
@@ -137,4 +137,184 @@ Proof.
         apply ble_nat_false in Heqle. apply Heqle.
 Qed.
 
+(* factorial:
+
+   loop invariant is Y * X! = m!
+
+   {{ X = m }} ->>                         (OK)
+   {{ 1 * X! = m! }}
+   Y ::= 1;
+   {{ Y * X! = m! }}
+   WHILE X <> 0 DO
+       {{ Y * X! = m! /\ X <> 0 }} ->>     (OK)
+       {{ Y * X * (X - 1)! = m! }}
+       Y ::= Y * X;
+       {{ Y * (X - 1)! = m! }}
+       X ::= X - 1;
+       {{ Y * X! = m! }}
+   END
+   {{ Y * X! = m! /\ ~(X <> 0) }} ->>      (OK)
+   {{ Y = m! }}
+*)
+
+(* min_hoare:
+
+   use:
+    Lemma lemma1: forall x y,
+        (x = 0) \/ (y = 0) -> min x y = 0.
+    Lemma lemma2: forall x y,
+        min (x - 1) (y - 1) = (min x y) - 1.
+
+    loop invariant is: min a b = (min X Y) + Z
+
+    {{ True }} ->>                             (OK)
+    {{ min a b = min a b}}
+    X ::= a;
+    {{ min a b = min X b }}
+    Y ::= b;
+    {{ min a b = min X Y }}
+    Z ::= 0;
+    {{ min a b = (min X Y) + Z }}
+    WHILE (X <> 0 /\ Y <> 0) DO
+        {{ min a b = (min X Y) + Z /\
+             (X <> 0 /\ Y <> 0)        }} ->>  (OK, lemma2)
+        {{ min a b = (min (X - 1) (Y - 1)) + Z + 1 }}
+        X ::= X - 1;
+        {{ min a b = (min X (Y - 1)) + Z + 1 }}
+        Y ::= Y - 1;
+        {{ min a b = (min X Y) + Z + 1 }}
+        Z ::= Z + 1;
+        {{ min a b = (min X Y) + Z }}
+    END
+    {{ min a b = (min X Y) + Z /\
+         ~( X <> 0 /\ Y <> 0)      }} ->>      (OK, lemma1)
+    {{ Z = min a b }}
+*)
+
+(* two_loops:
+
+   loop invariant is Z = X + Y + c
+
+   {{ True }} ->>                              (OK)
+   {{ c = c}}
+   X ::= 0;
+   {{ c = X + c }}
+   Y ::= 0;
+   {{ c = X + Y + c }}
+   Z ::= c;
+   {{ Z = X + Y + c }}
+   WHILE X <> a DO
+       {{ Z = X + Y + c /\ X <> a }} ->>       (OK)
+       {{ Z + 1 = X + 1 + Y + c }}
+       X ::= X + 1;
+       {{ Z + 1 = X + Y + c }}
+       Z ::= Z + 1;
+       {{ Z = X + Y + c }}
+   END
+   {{ Z = X + Y + c /\ X = a }} ->>            (OK)
+   {{ Z = a + Y + c }}
+   WHILE Y <> b DO
+       {{ Z = a + Y + c /\ Y <> b }} ->>       (OK)
+       {{ Z + 1 = a + Y + 1 + c }}
+       Y ::= Y + 1;
+       {{ Z + 1 = a + Y + c }}
+       Z ::= Z + 1;
+       {{ Z = a + Y + c }}
+   END
+   {{ Z = a + Y + c /\ Y = b }} ->>            (OK)
+   {{ Z = a + b + c }}
+*)
+
+(* dpow2_down:
+
+   power series: ( 1 + 2 + 2^2 + ... + 2^m = 2^(m+1) - 1 )
+
+   loop invariant is Y + 2*Z = 2^(X+2) - 1
+
+   {{ True }} ->>                                   (OK)
+   {{ 3 = 4 - 1}}
+   X ::= 0;
+   {{ 3 = 2^(X+2) - 1 }}
+   Y ::= 1;
+   {{ Y + 2 = 2^(X+2) -1 }}
+   Z ::= 1;
+   {{ Y + 2*Z = 2^(X+2) - 1 }}
+   WHILE X <> m DO
+       {{ Y + 2*Z = 2^(X+2) - 1 /\ X <> m }} ->>    (OK)
+       {{ Y + 2*Z + 2*2*Z = 2^(X+3) - 1 }}
+       Z ::= 2 * Z;
+       {{ Y + Z + 2*Z = 2^(X+3) - 1 }}
+       Y ::= Y + Z;
+       {{ Y + 2*Z = 2^(X+3) - 1 }}
+       X ::= X + 1;
+       {{ Y + 2*Z = 2^(X+2) - 1 }}
+   END
+   {{ Y + 2*Z = 2^(X+2) - 1 /\ X = m }} ->>         (OK)
+   {{ Y + 2*Z = 2^(m+2) - 1 }} ->>                  (OK)
+   {{ Y = 2^(m+1) - 1 }}
+*)
+
+Definition is_wp P c Q :=
+    {{ P }} c {{ Q }} /\
+    forall P', {{ P' }} c {{ Q }} -> (P' ->> P).
+
+Theorem is_pw_example:
+    is_wp (fun st => st Y <= 4)
+          (X ::= APlus (AId Y) (ANum 1))
+          (fun st => st X <= 5).
+Proof.
+    split.
+    Case "valid precodition".
+        eapply hoare_consequence_pre.
+        SCase "assignment".
+            apply hoare_asgn.
+        SCase "weaken precodition".
+            unfold assn_sub, assert_implies, update. simpl.
+            intros st H. omega.
+    Case "weakest precondition".
+        intros P' Htriple. unfold assert_implies. intros st HP'.
+        unfold hoare_triple in Htriple.
+        (* we need to build hypothesis
+           H : (X ::= APlus (AId Y) (ANum 1)) / st || st'
+           and use it with Htriple *)
+        remember (update st X (st Y + 1)) as st'.
+        assert (H: ((X ::= APlus (AId Y) (ANum 1)) / st || st')).
+            subst st'. apply E_Ass. simpl. reflexivity.
+        apply Htriple in H;
+            try assumption. (* (P' st) part in Htriple *)
+        rewrite Heqst' in H. unfold update in H. simpl in H. omega.
+Qed.
+
+Theorem hoare_sgn_weakest: forall Q X a,
+    is_wp (Q [X |-> a]) (X ::= a) Q.
+Proof.
+    intros Q X a. unfold is_wp. split.
+    Case "valid precondition".
+        apply hoare_asgn.
+    Case "weakest precondition".
+        intro P'. unfold assert_implies. intros Htriple st HP'.
+        unfold assn_sub. unfold hoare_triple in Htriple.
+        remember (update st X (aeval st a)) as st'.
+        apply Htriple with (st:= st).
+        subst st'. apply E_Ass. reflexivity.
+        assumption.
+Qed.
+
+Module Himp2.
+Import Himp.
+
+Lemma hoare_havoc_weakest: forall (P Q : Assertion) (X : id),
+    {{ P }} HAVOC X {{ Q }} ->
+    P ->> havoc_pre X Q.
+Proof.
+    intros P Q X Htriple. unfold assert_implies. intros st HP.
+    unfold havoc_pre. intro n. unfold hoare_triple in Htriple.
+    remember (update st X n) as st'.
+    apply Htriple with (st:=st);
+        try assumption.  (* (P st) part in Htriple *)
+    subst st'. apply E_Havoc.
+Qed.
+
+End Himp2.
+
 
